LeanProjeto2/StarLanguage/Axioms2.lean
@@ -25,8 +25,11 @@ open Batteries
 -- --------------------------------------
 -- --------------------------------------
 
-
 namespace Axioms
+
+/- ---------------------------------------------------------------
+                  AXIOMS FOR VARIABLES (matrices)
+-/ ---------------------------------------------------------------
 
 def AxiomE1_matrix (x : String) : Formula :=
   (var x)=₁(var x)
@@ -36,6 +39,7 @@ def AxiomUn_matrix (x : String) (t : String) (A : Formula) : Formula :=
   (b∀₁₁ x (var t) A) ↔₁ (∀₁₁ x (((var x) ∈₁ (var t)) →₁ A))
 def AxiomC1_matrix (x₁ x₂ : String) : Formula :=
   ((Π₁·(var x₁))·(var x₂)) =₁ (var x₁)
+--def AxiomC1_matrix (x₁ x₂ : String) : Formula := AxiomC1_matrix_ (.var x₁) (.var x₂)
 def AxiomC2_matrix (x₁ x₂ x₃ : String) : Formula :=
   (((Σ₁·(var x₁))·(var x₂))·(var x₃)) =₁ (((var x₁)·(var x₃))·((var x₂)·(var x₃)))
 def AxiomP1_matrix (x₁ x₂ : String) : Formula :=
@@ -51,6 +55,47 @@ def AxiomS3_matrix (x₁ x₂ x₃ y : String) : Formula :=
 def AxiomS4_matrix (x₁ x₂ : String) : Formula :=
   b∃₁₁ x₂ (var x₁) ((var x₂) ∈₁ (var x₁))
 
+/- ---------------------------------------------------------------
+              CORRESPONDING AXIOMS FOR TERMS (matrices)
+-/ ---------------------------------------------------------------
+
+@[reducible, simp]
+def AxiomE1_matrix_term (t : Term) : Formula :=
+  t=₁t
+@[reducible, simp]
+def AxiomE2_matrix_term (x : String) (t : Term) (A : Formula) (hA : isBase A) : Formula :=
+  (((var x)=₁t) ∧₁ A) →₁ (A.subst (HashMap.ofList ([x].zip ([t]))))
+@[reducible, simp]
+def AxiomUn_matrix_term (x : String) (t : Term) (A : Formula) : Formula :=
+  (b∀₁₁ x t A) ↔₁ (∀₁₁ x (((var x) ∈₁ t) →₁ A))
+@[reducible, simp]
+def AxiomC1_matrix_term (t₁ t₂ : Term) : Formula :=
+  ((Π₁·t₁)·t₂) =₁ t₁
+@[reducible, simp]
+def AxiomC2_matrix_term (t₁ t₂ t₃ : Term) : Formula :=
+  (((Σ₁·t₁)·t₂)·t₃) =₁ ((t₁·t₃)·(t₂·t₃))
+@[reducible, simp]
+def AxiomP1_matrix_term (t₁ t₂ : Term) : Formula :=
+  ((ind_⋃₁·(𝔰₁·t₁))·t₂) =₁ (t₂·t₁)
+@[reducible, simp]
+def AxiomP2_matrix_term (t₁ t₂ t₃ : Term) : Formula :=
+  ((ind_⋃₁·((∪₁·t₁)·t₂))·t₃) =₁ ((∪₁·((ind_⋃₁·t₁)·t₃))·((ind_⋃₁·t₂)·t₃))
+@[reducible, simp]
+def AxiomS1_matrix_term (t₁ t₂ : Term) : Formula :=
+  (t₁ ∈₁ (𝔰₁·t₂)) ↔₁ (t₁ =₁ t₂)
+@[reducible, simp]
+def AxiomS2_matrix_term (t₁ t₂ t₃ : Term) : Formula :=
+  (t₁ ∈₁ ((∪₁·t₂)·t₃) ) ↔₁ ((t₁ ∈₁ t₂) ∨₁ (t₁ ∈₁ t₃))
+@[reducible, simp]
+def AxiomS3_matrix_term (t₁ t₂ t₃ : Term) (y : String) : Formula :=
+  (t₃ ∈₁ ((ind_⋃₁·t₁)·t₂)) ↔₁ (b∃₁₁ y t₁ (t₃ ∈₁ (t₂·(var y))))
+@[reducible, simp]
+def AxiomS4_matrix_term (x : String) (t : Term) : Formula :=
+  b∃₁₁ x t ((var x) ∈₁ t)
+
+
+-- ------------------------------------------------------------------------
+-- ------------------------------------------------------------------------
 
 -- LEMMA: substituir não altera baseness
 lemma Subst_isBase (A : Formula) (hA : isBase A) (x : List String) (t : List Term) : isBase (A.subst (HashMap.ofList (x.zip t))) := by
@@ -150,24 +195,24 @@ lemma AxiomS4_univ_of_base : (isBase (AxiomS4_matrix x₁ x₂)) := by
 
 -- ---------------------------------------------------------------
 
+/- ---------------------------------------------------------------
+      UNIVERSAL CLOSURE OF THE MATRICES FROM BEFORE (variables)
+-/ ---------------------------------------------------------------
+
 def AxiomE1 (x : String) : Formula :=
   ∀₁₁ x (AxiomE1_matrix x)
 def AxiomE2 (x₁ x₂ : String) (A : Formula) (hA : isBase A) : Formula :=
   ∀₁₁ x₁ (∀₁₁ x₂ (AxiomE2_matrix x₁ x₂ A hA))
--- ---
 def AxiomUn (x : String) (t : String) (A : Formula) : Formula :=
   ∀₁₁ t (AxiomUn_matrix x t A)
--- ----
 def AxiomC1 (x₁ x₂ : String) : Formula :=
   ∀₁₁ x₁ (∀₁₁ x₂ (AxiomC1_matrix x₁ x₂))
 def AxiomC2 (x₁ x₂ x₃ : String) : Formula :=
   ∀₁₁ x₁ (∀₁₁ x₂ (∀₁₁ x₃ (AxiomC2_matrix x₁ x₂ x₃)))
--- ----
 def AxiomP1 (x₁ x₂ : String) : Formula :=
   ∀₁₁ x₁ (∀₁₁ x₂ (AxiomP1_matrix x₁ x₂))
 def AxiomP2 (x₁ x₂ x₃ : String) : Formula :=
   ∀₁₁ x₁ (∀₁₁ x₂ (∀₁₁ x₃ (AxiomP2_matrix x₁ x₂ x₃)))
--- ----
 def AxiomS1 (x₁ x₂ : String) : Formula :=
   ∀₁₁ x₁ (∀₁₁ x₂ (AxiomS1_matrix x₁ x₂))
 def AxiomS2 (x₁ x₂ x₃ : String) : Formula :=
@@ -253,19 +298,33 @@ inductive ProvableFrom : Set Formula → Formula → Prop
 | AxS₃:                       Γ ⊢ AxiomS3 x₁ x₂ x₃ y
 | AxS₄:                       Γ ⊢ AxiomS4 x₁ x₂
 
+
 /-
-| AxE₁ (t:Term) :                               Γ ⊢ (t=₁t)
-| AxE₂ (t₁ t₂ :Term) (hA : isBase A) :          Γ ⊢ ((t₁=₁t₂) ∧₁ (A →₁ A))     -- TBD: falta substituição aqui
-| AxU (x : String) (t : Term) (A : Formula) :   Γ ⊢ ((b∀₁₁ x t A) ↔₁ (∀₁₁ x (((var x) ∈₁ t) →₁ A)))
-| AxC₁ (t₁ t₂ : Term) :                         Γ ⊢ (((Π₁·t₁)·t₂) =₁ t₁)
-| AxC₂ (t₁ t₂ t₃ : Term) :                      Γ ⊢ ((((Σ₁·t₁)·t₂)·t₃) =₁ ((t₁·t₃)·(t₂·t₃)))
-| AxP₁ (t₁ t₂ : Term) :                         Γ ⊢ (((ind_⋃₁·(𝔰₁·t₁))·t₂) =₁ (t₂·t₁))
-| AxP₂ (t₁ t₂ t₃ : Term) :                      Γ ⊢ (((ind_⋃₁·((∪₁·t₁)·t₂))·t₃) =₁ ((∪₁·((ind_⋃₁·t₁)·t₃))·((ind_⋃₁·t₂)·t₃)))
-| AxS₁ (t₁ t₂ : Term) :                         Γ ⊢ ((t₁ ∈₁ (𝔰₁·t₂)) ↔₁ (t₁ =₁ t₂))
-| AxS₂ (t₁ t₂ t₃ : Term) :                      Γ ⊢ ((t₁ ∈₁ ((∪₁·t₂)·t₃) ) ↔₁ ((t₁ ∈₁ t₂) ∨₁ (t₁ ∈₁ t₃)))
-| AxS₃ (a f b : Term) :                         Γ ⊢ ((b ∈₁ ((ind_⋃₁·a)·f)) ↔₁ (b∃₁₁ x a (b ∈₁ (f·(var x)))))
+| AxE₁_term (t:Term) :                               Γ ⊢ (t=₁t)
+| AxE₂_term (t₁ t₂ :Term) (hA : isBase A) :          Γ ⊢ ((t₁=₁t₂) ∧₁ (A →₁ A))     -- TBD: falta substituição aqui
+| AxU_term (x : String) (t : Term) (A : Formula) :   Γ ⊢ ((b∀₁₁ x t A) ↔₁ (∀₁₁ x (((var x) ∈₁ t) →₁ A)))
+| AxC₁_term (t₁ t₂ : Term) :                         Γ ⊢ (((Π₁·t₁)·t₂) =₁ t₁)
+| AxC₂_term (t₁ t₂ t₃ : Term) :                      Γ ⊢ ((((Σ₁·t₁)·t₂)·t₃) =₁ ((t₁·t₃)·(t₂·t₃)))
+| AxP₁_term (t₁ t₂ : Term) :                         Γ ⊢ (((ind_⋃₁·(𝔰₁·t₁))·t₂) =₁ (t₂·t₁))
+| AxP₂_term (t₁ t₂ t₃ : Term) :                      Γ ⊢ (((ind_⋃₁·((∪₁·t₁)·t₂))·t₃) =₁ ((∪₁·((ind_⋃₁·t₁)·t₃))·((ind_⋃₁·t₂)·t₃)))
+| AxS₁_term (t₁ t₂ : Term) :                         Γ ⊢ ((t₁ ∈₁ (𝔰₁·t₂)) ↔₁ (t₁ =₁ t₂))
+| AxS₂_term (t₁ t₂ t₃ : Term) :                      Γ ⊢ ((t₁ ∈₁ ((∪₁·t₂)·t₃) ) ↔₁ ((t₁ ∈₁ t₂) ∨₁ (t₁ ∈₁ t₃)))
+| AxS₃_term (a f b : Term) :                         Γ ⊢ ((b ∈₁ ((ind_⋃₁·a)·f)) ↔₁ (b∃₁₁ x a (b ∈₁ (f·(var x)))))
 -- TBD: FALTA AXS4
 -/
+
+axiom AxE₁_term (Γ : Set Formula) (t:Term): Γ ⊢ (t=₁t)
+axiom AxE₂_term (Γ : Set Formula) (x x₁:String) (t :Term) (A:Formula) (hA : isBase A) :       Γ ⊢ (((var x₁)=₁t) ∧₁ (A →₁ (A.subst (HashMap.ofList ([x].zip [t])))))
+axiom AxU_term (Γ : Set Formula) (x : String) (t : Term) (A : Formula) :                      Γ ⊢ ((b∀₁₁ x t A) ↔₁ (∀₁₁ x (((var x) ∈₁ t) →₁ A)))
+axiom AxC₁_term (Γ : Set Formula) (t₁ t₂ : Term) :                                            Γ ⊢ (((Π₁·t₁)·t₂) =₁ t₁)
+axiom AxC₂_term (Γ : Set Formula) (t₁ t₂ t₃ : Term) :                                         Γ ⊢ ((((Σ₁·t₁)·t₂)·t₃) =₁ ((t₁·t₃)·(t₂·t₃)))
+axiom AxP₁_term (Γ : Set Formula) (t₁ t₂ : Term) :                                            Γ ⊢ (((ind_⋃₁·(𝔰₁·t₁))·t₂) =₁ (t₂·t₁))
+axiom AxP₂_term (Γ : Set Formula) (t₁ t₂ t₃ : Term) :                                         Γ ⊢ (((ind_⋃₁·((∪₁·t₁)·t₂))·t₃) =₁ ((∪₁·((ind_⋃₁·t₁)·t₃))·((ind_⋃₁·t₂)·t₃)))
+axiom AxS₁_term (Γ : Set Formula) (t₁ t₂ : Term) :                                            Γ ⊢ ((t₁ ∈₁ (𝔰₁·t₂)) ↔₁ (t₁ =₁ t₂))
+axiom AxS₂_term (Γ : Set Formula) (t₁ t₂ t₃ : Term) :                                         Γ ⊢ ((t₁ ∈₁ ((∪₁·t₂)·t₃) ) ↔₁ ((t₁ ∈₁ t₂) ∨₁ (t₁ ∈₁ t₃)))
+axiom AxS₃_term (Γ : Set Formula) (x:String) (a f b : Term) :                                 Γ ⊢ ((b ∈₁ ((ind_⋃₁·a)·f)) ↔₁ (b∃₁₁ x a (b ∈₁ (f·(var x)))))
+-- TBD: FALTA AXS4
+
 
 end
 
